Added some specs for ctr.Get();
One oddity: there are a couple of different specs.
E.g. a user of a ctr server might have `exists some_v, kv_ptsto_epoch k epoch some_v`, and want
to do a ctr.Get(epoch) to physically learn the value of some_v. Other
times, the caller of ctr.Get() might also have the end-user exposed
`kv_ptsto k v` and want to fire a fupd against that in addition to
`kv_ptsto_epoch`. At this point, I can't tell how to combine them.

src/program_proof/fencing/ctr_proof.v
@@ -4,34 +4,78 @@ From Perennial.program_proof Require Import grove_prelude.
 From Perennial.program_proof.memkv Require Export rpc_lib rpc_proof rpc_spec.
 
 Section ctr_definitions.
+Context `{!gooseGlobalGS Σ}.
 Context `{!heapGS Σ}.
 
 Record ctr_names :=
   {}.
 
-Definition kv_ptsto_epoch (k e v:u64) : iProp Σ.
+Definition kv_epoch_unknown (k e:u64) : iProp Σ.
+Admitted.
+
+Definition kv_epoch_ptsto (k e v:u64) : iProp Σ.
 Admitted.
 
 Definition kv_ptsto (k v:u64) : iProp Σ.
 Admitted.
 
-Definition own_Clerk : iProp Σ.
+Definition own_Clerk (ck:loc) : iProp Σ.
 Admitted.
 
 
 (* |={Eo,Ei}=> ∃ vold, kv_ptsto k vold ∗ (kv_ptsto k vnew ={Ei,Eo}=∗ Q) *)
 
-Lemma wp_Clerk__Put (γ:ctr_names) (k e v:u64):
-  {{{
-      (∃ oldv, kv_ptsto_epoch k e oldv) ∗
-      (∃ oldv2, kv_ptsto k oldv2)
-  }}}
-    Clerk__Put #v #e
-  {{{
-        RET #(); kv_ptsto k v
-  }}}.
+(* XXX: the current Clerk is a sequential clerk: can only do one operation at a
+   time with it. Will need to have multiple CIDs to do multiple operations. *)
+
+Lemma wp_Clerk__Put_typical {Eo Ei:coPset} Φ (k v:u64):
+  (|={Eo,Ei}=> ∃ vold, kv_ptsto k vold ∗ (kv_ptsto k v ={Ei,Eo}=∗ Φ #v)) -∗
+    WP Clerk__Put #() @ Eo {{ Φ }}.
 Proof.
-  iIntros (Φ) "Hpre HΦ".
 Admitted.
+
+Lemma wp_Clerk__Put {Eo Ei:coPset} Φ (k e v:u64):
+  (|={Eo,Ei}=> ∃ vold, kv_ptsto k vold ∗ kv_epoch_ptsto k e vold ∗
+    (kv_ptsto k v ∗ kv_epoch_ptsto k e v ={Ei,Eo}=∗ Φ #v)) -∗
+    WP Clerk__Put #() @ Eo {{ Φ }}.
+Proof.
+Admitted.
+
+Lemma wp_Clerk__Put_unknown {Eo Ei:coPset} Φ (k e v:u64):
+  (|={Eo,Ei}=> ∃ vold, kv_ptsto k vold ∗ kv_epoch_unknown k e ∗
+    (kv_ptsto k v ∗ kv_epoch_ptsto k e v ={Ei,Eo}=∗ Φ #v)) -∗
+    WP Clerk__Put #() @ Eo {{ Φ }}.
+Proof.
+Admitted.
+
+Lemma wp_Clerk__Get_unknown {Eo Ei:coPset} ck (k e:u64):
+  ∀ Φ,
+  own_Clerk ck -∗
+  (|={Eo,Ei}=> ∃ v, kv_ptsto k v ∗ kv_epoch_unknown k e ∗
+    (kv_ptsto k v ∗ kv_epoch_ptsto k e v ={Ei,Eo}=∗ (own_Clerk ck -∗ Φ #v))) -∗
+    WP Clerk__Get #() @ Eo {{ Φ }}.
+Proof.
+Admitted.
+
+Lemma wp_Clerk__Get_unknown_epoch_only {Eo Ei:coPset} ck (k e:u64):
+  ∀ Φ,
+  own_Clerk ck -∗
+            (|={Eo,Ei}=> ∃ v, kv_epoch_unknown k e ∗ (kv_epoch_ptsto k e v ={Ei,Eo}=∗
+                                                              (own_Clerk ck -∗ Φ #v))) -∗
+    WP Clerk__Get #ck #e @ Eo {{ Φ }}.
+Proof.
+Admitted.
+
+(*
+Lemma wp_Server__Put {Eo Ei:coPset} Φ (k e v:u64) (s args:loc):
+  (|={Eo,Ei}=> ∃ vold, kv_ptsto k vold ∗ kv_ptsto_epoch k e vold ∗
+    (kv_ptsto k v ∗ kv_ptsto_epoch k e v ={Ei,Eo}=∗ Φ #v)) -∗
+    WP Server__Put #s #args @ Eo {{ Φ }}.
+Proof.
+  iIntros "Hpre".
+  wp_lam.
+  wp_pures.
+  (* wp_loadField. *)
+Admitted. *)
 
 End ctr_definitions.
