src/program_proof/fencing/frontend_proof.v
@@ -1,0 +1,57 @@
+From Perennial.program_proof Require Import grove_prelude.
+From Goose.github_com.mit_pdos.gokv.fencing Require Import frontend.
+From Perennial.program_proof Require Import grove_prelude.
+From Perennial.program_proof.memkv Require Export rpc_lib rpc_proof rpc_spec.
+
+Section frontend_proof.
+
+Context `{!heapGS Σ}.
+
+Definition own_Server (s:loc) epoch : iProp Σ :=
+  ∃ ck1 ck2,
+  "#Hepoch" ∷ readonly (s ↦[frontend.Server :: "epoch"] #epoch) ∗
+  "Hck1" ∷ s ↦[frontend.Server :: "ck1"] #ck1 ∗
+  "Hck2" ∷ s ↦[frontend.Server :: "ck1"] #ck2 ∗
+  (* TODO: add ownership of clerks *)
+  "_" ∷ True.
+
+Definition frontendN := nroot .@ "frontend".
+
+Definition is_Server s : iProp Σ :=
+  ∃ mu,
+  "Hmu" ∷ readonly (s ↦[frontend.Server :: "mu"] mu) ∗
+  "HmuInv" ∷ is_lock frontendN mu (∃ epoch, own_Server s epoch)
+.
+
+Lemma wp_FetchAndIncrement (s:loc) (key:u64) :
+  key = 0 ∨ key = 1 →
+  is_Server s -∗
+  {{{
+        True
+  }}}
+    Server__FetchAndIncrement #s #key
+  {{{
+        (v:u64), RET #v; True
+  }}}.
+Proof.
+  intros Hkey.
+  iIntros "#Hsrv !#" (Φ) "_ HΦ".
+  wp_lam.
+  wp_pures.
+  iNamed "Hsrv".
+  wp_loadField.
+  wp_apply (acquire_spec with "HmuInv").
+  iIntros "[Hlocked Hown]".
+  iNamed "Hown".
+  wp_pures.
+  wp_apply (wp_ref_of_zero).
+  { done. }
+  iIntros (Hret_ptr) "Hret".
+  wp_pures.
+  wp_if_destruct.
+  {
+    wp_loadField.
+    wp_loadField.
+    wp_apply (wp_Clerk__Get_unknown).
+  }
+End frontend_proof.
